simplify precondition of mul1_add

code/experimental/curve25519/Hacl.Spec.Curve25519.Field64.Core.fst
@@ -172,10 +172,12 @@ val mul1_add:
   -> u2:uint64
   -> f3:felem4
   -> Pure (uint64 & felem4)
-    (requires as_nat4 f3 + as_nat4 f1 * v u2 < pow2 320)
+    (requires True)
     (ensures fun (c, r) ->
       as_nat4 r + v c * pow2 256 == as_nat4 f3 + as_nat4 f1 * v u2)
 let mul1_add f1 u2 f3 =
+  lemma_mul1_add_pre f1 u2 f3;
+  assert (as_nat4 f3 + as_nat4 f1 * v u2 < pow2 320);
   let c, out0 = mul1 f1 u2 in
   let (o0, o1, o2, o3) = out0 in
   let (f30, f31, f32, f33) = f3 in
@@ -304,18 +306,23 @@ val mul4:
     f1:felem4
   -> r:felem4
   -> out:felem_wide4{wide_as_nat4 out == as_nat4 f1 * as_nat4 r}
-let mul4 f1 r = admit();
+let mul4 f1 r =
   let (f0, f1, f2, f3) = f1 in
   let c0, out0 = mul1 r f0 in
+  assert (as_nat4 out0 + v c0 * pow2 256 == as_nat4 r * v f0);
   let (o00, o01, o02, o03) = out0 in
   let c1, out1 = mul1_add r f1 (o01, o02, o03, c0) in
+  assert (as_nat4 out1 + v c1 * pow2 256 == as_nat4 (o01, o02, o03, c0) + as_nat4 r * v f1);
   let (o11, o12, o13, o14) = out1 in
   let c2, out2 = mul1_add r f2 (o12, o13, o14, c1) in
+  assert (as_nat4 out2 + v c2 * pow2 256 == as_nat4 (o12, o13, o14, c1) + as_nat4 r * v f2);
   let (o22, o23, o24, o25) = out2 in
   let c3, out3 = mul1_add r f3 (o23, o24, o25, c2) in
+  assert (as_nat4 out3 + v c3 * pow2 256 == as_nat4 (o23, o24, o25, c2) + as_nat4 r * v f3);
   let (o33, o34, o35, o36) = out3 in
   let o37 = c3 in
   let out = (o00, o11, o22, o33, o34, o35, o36, o37) in
+    admit();
   out
 
 val fmul4:
